\documentclass[twocolumn, 10pt]{article}
\usepackage[a4paper, margin=10pt]{geometry}
\usepackage{enumitem}
\usepackage{amsmath}
\usepackage{graphicx}
\usepackage{xcolor}
\usepackage{tabularray}
\usepackage{mathtools}

\setlength{\parindent}{0pt}

\begin{document}

\MakeUppercase{\textbf{\Large Regras de Derivação}}

\vspace{8pt}
\MakeUppercase{Derivadas Simples}

\begin{itemize}[topsep=2pt]
    \item Soma/Diferença: $\left(f \pm g\right)' = f' \pm g'$
    \item Produto: $\left(fg\right)' = f'g + fg'$ \\[2pt]
        Constante: $\left(\alpha f\right)' = \alpha f'$
    \item Quociente: 
        $\displaystyle \left(\frac{f}{g}\right)' = \frac{f'g - fg'}{g^2}$
    \item Potência: $\displaystyle \left(f^\alpha\right)' = \alpha f^{\alpha - 1}f'$
    \item Exponencial: 
        $\displaystyle \left(\alpha^f\right)' = f' a^f (\ln \alpha)$ \\[2pt]
        Base $e$: $\displaystyle \left(e^f\right)' = f' e^f$
    \item Logaritmo: 
        $\displaystyle \left(\log_{\alpha} f\right)' = \frac{f'}{f (\ln \alpha)}$ \\[2pt]
        Base $e$: $\displaystyle \left(\ln f\right)' = \frac{f'}{f}$
    \item Funções Trigonométricas:
        \begin{itemize}[topsep=0pt]
            \item $(\sin f)' = f' (\cos f)$
            \item $(\cos f)' = -f' (\sin f)$
            \item $\displaystyle (\tan f)' = \frac{f'}{\cos^2 f}$
            \item $\displaystyle (\arcsin f)' = \frac{f'}{\sqrt{1-f^2}}$
            \item $\displaystyle (\arccos f)' = -\frac{f'}{\sqrt{1-f^2}}$
            \item $\displaystyle (\arctan f)' = \frac{f'}{1 + f^2}$
        \end{itemize}
    \item Função Hiperbólicas:
        \begin{itemize}[topsep=0pt]
            \item $(\sinh f)' = f' (\cosh f)$
            \item $(\cosh f)' = f' (\sinh f)$
        \end{itemize}
\end{itemize}

\vspace{8pt}
\MakeUppercase{Derivada da Função Composta}

\begin{itemize}[topsep=2pt]
    \item $f\left[g(x)\right]' = f'\left[g(x)\right] \times g'(x) $
\end{itemize}

\vspace{8pt}
\MakeUppercase{Derivada da Função Inversa}

\begin{itemize}[topsep=2pt]
    \item $\displaystyle \left(f^{-1}\right)'(y) = \frac{1}{f'\left(f^{-1}(y)\right)}$
\end{itemize}

\newpage

\MakeUppercase{\textbf{\Large Regras de Primitivação}}

\vspace{8pt}
\MakeUppercase{Primitivas Imadiatas e Quase-Imediatas}

\begin{itemize}[topsep=2pt]
    \item 
\end{itemize}

\vspace{8pt}
\MakeUppercase{Primitivação por partes}

\begin{itemize}[topsep=2pt]
    \item $\displaystyle \int u(x)\cdot v'(x)\,dx = u(x) \cdot v(x) - \int u'(x) \cdot v(x)\,dx$
\end{itemize}

\vspace{8pt}
\MakeUppercase{Primitivação por substituição}

\begin{itemize}
    \item $\displaystyle \int f(x)\,dx = \left(\int f(u(t))\,u'(t)\,dt\right)_{t=u^{-1}(x)}$
\end{itemize}

\end{document}